Weidenbach_Book/IsaSAT/IsaSAT_VMTF.thy
@@ -535,23 +535,6 @@ lemma isa_vmtf_mark_to_rescore_vmtf_mark_to_rescore:
   by (intro frefI nres_relI)
     (auto intro!: atoms_hash_del_op_set_insert[THEN fref_to_Down_unRET_uncurry])
 *)
-definition (in -) isa_vmtf_unset :: \<open>nat \<Rightarrow> vmtf \<Rightarrow> vmtf\<close> where
-\<open>isa_vmtf_unset = (\<lambda>L (ns, m, fst_As, lst_As, next_search).
-  (if next_search = None \<or> stamp (ns ! (the next_search)) < stamp (ns ! L)
-  then ((ns, m, fst_As, lst_As, Some L))
-  else ((ns, m, fst_As, lst_As, next_search))))\<close>
-
-definition vmtf_unset_pre where
-\<open>vmtf_unset_pre = (\<lambda>L (ns, m, fst_As, lst_As, next_search).
-  L < length ns \<and> (next_search \<noteq> None \<longrightarrow> the next_search < length ns))\<close>
-
-lemma vmtf_unset_pre_vmtf:
-  assumes
-    \<open>((ns, m, fst_As, lst_As, next_search)) \<in> vmtf \<A> M\<close> and
-    \<open>L \<in># \<A>\<close>
-  shows \<open>vmtf_unset_pre L ((ns, m, fst_As, lst_As, next_search))\<close>
-  using assms
-  by (auto simp: vmtf_def vmtf_unset_pre_def atms_of_\<L>\<^sub>a\<^sub>l\<^sub>l_\<A>\<^sub>i\<^sub>n)
 
 definition isa_vmtf where
   \<open>isa_vmtf \<A> M =
