Weidenbach_Book/IsaSAT/IsaSAT_VMTF_LLVM.thy
@@ -542,22 +542,22 @@ sepref_def vmtf_mark_to_rescore_also_reasons_fast_code
   unfolding  nres_monad3 case_option_split
   by sepref
 
-lemma isa_vmtf_mark_to_rescore_also_reasons_clD:
+lemma isa_vmtf_bump_to_rescore_also_reasons_clD:
   \<open>arena_is_valid_clause_idx arena C \<Longrightarrow> C + arena_length arena C \<le> length arena\<close>
   apply (auto simp: arena_is_valid_clause_idx_def arena_lifting)
   using arena_lifting(10) arena_lifting(4) by auto
 
-sepref_register  isa_vmtf_mark_to_rescore_also_reasons_cl
-sepref_def isa_vmtf_mark_to_rescore_also_reasons_cl_impl
-  is \<open>uncurry4 (isa_vmtf_mark_to_rescore_also_reasons_cl)\<close>
+sepref_register  isa_vmtf_bump_to_rescore_also_reasons_cl
+sepref_def isa_vmtf_bump_to_rescore_also_reasons_cl_impl
+  is \<open>uncurry4 (isa_vmtf_bump_to_rescore_also_reasons_cl)\<close>
   :: \<open>[\<lambda>((((_, N), _), _), _). length N \<le> sint64_max]\<^sub>a
   trail_pol_fast_assn\<^sup>k *\<^sub>a arena_fast_assn\<^sup>k *\<^sub>a sint64_nat_assn\<^sup>k *\<^sub>a unat_lit_assn\<^sup>k *\<^sub>a vmtf_remove_assn\<^sup>d \<rightarrow>
   vmtf_remove_assn\<close>
   supply image_image[simp] uminus_\<A>\<^sub>i\<^sub>n_iff[iff] in_diffD[dest] option.splits[split]
     in_\<L>\<^sub>a\<^sub>l\<^sub>l_atm_of_\<A>\<^sub>i\<^sub>n[simp]
   supply [[goals_limit=1]]
-  supply [dest] = isa_vmtf_mark_to_rescore_also_reasons_clD
-  unfolding isa_vmtf_mark_to_rescore_also_reasons_cl_def PR_CONST_def
+  supply [dest] = isa_vmtf_bump_to_rescore_also_reasons_clD
+  unfolding isa_vmtf_bump_to_rescore_also_reasons_cl_def PR_CONST_def
   unfolding while_eq_nfoldli[symmetric]
   apply (subst while_upt_while_direct, simp)
   apply (annot_snat_const \<open>TYPE(64)\<close>)
@@ -603,7 +603,7 @@ export_llvm
   vmtf_rescore_fast_code
   vmtf_mark_to_rescore_clause_fast_code
   vmtf_mark_to_rescore_also_reasons_fast_code
-  isa_vmtf_mark_to_rescore_also_reasons_cl_impl
+  isa_vmtf_bump_to_rescore_also_reasons_cl_impl
 end
 
 end
